

IFT-2125 assignment #1

Tarik Hireche | 202 301 89

04. March 2025

1 Asymptotic notation (25 points)

Question 1

We are asked to prove or refute the following propositions:

1. $\lfloor \frac{n}{2} \rfloor \in O(\sqrt{n})$
2. $n\sqrt{n} \log(n!) \in O(n^3 \log(n))$

Let's start with the first proposition, $\lfloor \frac{n}{2} \rfloor \in O(\sqrt{n})$:

Intuitively, this proposition is false because when n is very large $\lfloor \frac{n}{10} \rfloor \approx \frac{n}{10}$.

Let's prove this rigorously. Suppose that $\lfloor \frac{n}{10} \rfloor \in O(\sqrt{n})$, then by the definition of the big O notation:

$$(\exists c \in \mathbb{R}^{\geq 0}), (\exists n_0 \in \mathbb{N}) : \forall n \geq n_0, \left\lfloor \frac{n}{10} \right\rfloor \leq c \cdot \sqrt{n} \quad (1.1)$$

Also, we can see that:

$$\frac{n}{10} - 1 \leq \left\lfloor \frac{n}{10} \right\rfloor \leq \frac{n}{10} \quad (*) \quad (1.2)$$

So $\frac{n}{2} - 1$ constitutes a lower bound for $\lfloor \frac{n}{10} \rfloor$ and $\frac{n}{2}$ is an upper bound for $\lfloor \frac{n}{10} \rfloor$.

That means that $\lfloor \frac{n}{10} \rfloor$ is at most $\frac{n}{10}$. We are going to use that fact.

Great, now let's setup the equation and do a bit of mental gymnastics. We have that:

$$\left\lfloor \frac{n}{10} \right\rfloor \leq c \cdot \sqrt{n} \quad (1.3)$$

$$\left\lfloor \frac{n}{10} \right\rfloor \leq c \cdot n^{\frac{1}{2}} \quad (1.4)$$

We saw earlier that $\lfloor \frac{n}{2} \rfloor \geq \frac{n}{2} - 1$, so using (*) this would imply:

$$\frac{n}{10} - 1 \leq c \cdot n^{\frac{1}{2}} \quad (1.5)$$

For very large n , the term -1 becomes negligible. So we have:

$$\frac{n}{10} \leq c \cdot n^{\frac{1}{2}} \quad (1.6)$$

$$\frac{1}{10} \cdot n \leq c \cdot n^{\frac{1}{2}} \quad (1.7)$$

$$\frac{1}{n^{\frac{1}{2}}} \cdot \left(\frac{1}{10} \cdot n \right) \leq \frac{1}{n^{\frac{1}{2}}} \cdot (c \cdot n^{\frac{1}{2}}) \quad (1.8)$$

$$\frac{1}{10} \cdot n^{1-\frac{1}{2}} \leq c \cdot n^{\frac{1}{2}-\frac{1}{2}} \quad (1.9)$$

$$\frac{1}{10} \cdot \sqrt{n} \leq c \quad (1.10)$$

$$\sqrt{n} \leq 10c \quad (1.11)$$

$$n \leq (10c)^2 \quad (1.12)$$

Let's set $(10c)^2 = d$, that means that:

$$n \leq d, \text{ où } d \in \mathbb{N} \quad (1.13)$$

$$\rightarrow \leftarrow \text{Contradiction.} \quad (1.14)$$

By supposing that $\lfloor \frac{n}{2} \rfloor \in O(\sqrt{n})$, we have stumbled upon a contradiction. Why? Well it is because n cannot have an upper bound because by definition, the condition must hold for all $n \geq n_0$, the threshold. Therefore:

$$\left\lfloor \frac{n}{2} \right\rfloor \notin O(\sqrt{n})$$

$$2. \ n\sqrt{n} \log(n!) \in O(n^3 \log(n))$$

After giving some thoughts about this, I want to explore an interesting property of the big O notation to demonstrate the proposition. I am going to use the following property viewed in class and available in the chapter #3 titled *Asymptotic Notation p.10* :

$$f_1(n) \in O(g_1(n)) \wedge f_2(n) \in O(g_2(n)) \rightarrow f_1(n) \cdot f_2(n) \in O(g_1(n) \cdot g_2(n))$$

$$\text{Let } f_1(n) = n\sqrt{n}, \ f_2(n) = \log(n!), \ g_1(n) = n^3, \ g_2(n) = \log(n)$$

Okay, we have a bunch of work to do now.

I) Let's show that $f_1(n) \in O(g_1(n))$.

If $n\sqrt{n} \in O(n^3)$, then by the definition:

$$(\exists c \in \mathbb{R}^{\geq 0}), (\exists n_0 \in \mathbb{N}) : \forall n \geq n_0, n\sqrt{n} \leq c \cdot n^3 \quad (1.1)$$

$$n\sqrt{n} \leq c \cdot n^3 \quad (1.2)$$

$$\frac{1}{n} \cdot (n\sqrt{n}) \leq \frac{1}{n} \cdot (c \cdot n^3) \quad (1.3)$$

$$n^{\frac{1}{2}} \leq c \cdot n^2 \quad (1.4)$$

$$1 \leq c \cdot n^{2-\frac{1}{2}} \quad (1.5)$$

$$\frac{1}{c} \leq n^{\frac{3}{2}} \quad (1.6)$$

We raise both sides of inequality (1.6) to the power of $\frac{2}{3}$ to isolate n . This operation leaves us with:

$$n \geq \frac{1}{c^{\frac{2}{3}}} \quad (1.7)$$

We have found a threshold $n_0 = \frac{1}{c^3}$ from which $n^3 \geq n\sqrt{n}$ with $c = 1$. With this, we can conclude that:

$$n\sqrt{n} \in O(n^3) \quad (1.8)$$

II) Let's show that $f_2(n) \in O(g_2(n))$.

If $\log(n!) \in O(\log(n))$, then by the definition:

$$(\exists c \in \mathbb{R}^{\geq 0}), (\exists n_{0'} \in \mathbb{N}) : \forall n \geq n_{0'}, \log(n!) \leq c' \cdot \log(n) \quad (1.9)$$

$\log(n!)$ is somewhat abstract to visualize isn't it? Let's find a way to make it clearer to understand.

First of all, we can observe that

$$\log(n!) = \log[n \times (n-1) \times (n-2) \times \dots \times 3 \times 2 \times 1] \quad (1.10)$$

$$= \log(n) + \log(n-1) + \dots + \log(3) + \log(2) + \log(1) \quad (1.11)$$

We have seen a similar exercise in class that splits this sum in half and I am going to use the same idea to find a lower bound for $\log(n!)$.

Let's call this lower bound function $f_{lb}(n)$. If $f_{lb}(n)$ is a lower bound for $\log(n!)$ that means:

$$f_{lb}(n) \leq \log(n!) \quad (1.12)$$

Which also means that $f_{lb}(n)$ has to also be in $O(\log(n))$ if $\log(n!)$ is.

Let's find $f_{lb}(n)$:

$$\log(n!) = \log(n) + \log(n-1) + \dots + \log(3) + \log(2) + \log(1) \quad (1.13)$$

$$= \sum_{i=1}^n \log(i) \quad (1.14)$$

Let's split the sum in half, the first half S_{n_1} from $[1, n/2]$ and the second half S_{n_2} from $[\frac{n}{2} + 1, n]$:

$$S_{n_1} = \sum_{i=1}^{\lfloor \frac{n}{2} \rfloor} \log(i), \quad S_{n_2} = \sum_{i=\lfloor \frac{n}{2} \rfloor + 1}^n \log(i) \quad (1.15)$$

Of course this makes it obvious that:

$$\log(n!) = S_{n_1} + S_{n_2} \quad (1.16)$$

Every term in S_{n_2} is at least $\log(\frac{n}{2})$ as the sum starts from $i = \frac{n}{2} + 1$ and since we split our sum in half then there are $\frac{n}{2}$ terms in the second sum; $|\{S_{n_2}\}| = n - (\frac{n}{2} + 1) + 1 = \frac{n}{2}$.

$$\text{We can therefore use } \frac{n}{2} \times \log\left(\frac{n}{2}\right) \text{ as a lower bound for } \log(n!) : \quad (1.17)$$

$$\frac{n}{2} \cdot \log\left(\frac{n}{2}\right) \leq \log(n!) \quad (1.18)$$

if $\frac{n}{2} \cdot \log(\frac{n}{2})$ is a lower bound for $\log(n!)$ then it must be in $O(\log(n))$ as well. Let's play around with:

$$\frac{n}{2} \cdot \log\left(\frac{n}{2}\right) \leq c' \cdot \log(n) \quad (1.19)$$

$$\frac{\frac{n}{2} \cdot \log(\frac{n}{2})}{\log(n)} \leq c' \cdot \frac{\log(n)}{\log(n)} \quad (1.20)$$

$$\frac{n}{2} \cdot \frac{\log(\frac{n}{2})}{\log(n)} \leq c' \quad (1.21)$$

For large n , $\frac{\log(\frac{n}{2})}{\log(n)} \rightarrow 1$ as the coefficient $\frac{1}{2}$ becomes negligible, therefore the equation becomes:

$$\frac{n}{2} \leq c' \quad (1.22)$$

$$n \leq 2c' \quad (1.23)$$

$$\rightarrow \leftarrow \text{Contradiction} \quad (1.24)$$

Even if we did not clean up the expression, the contradiction had already risen up (at the *line (1.20)*). We had on the left side an expression that is a lower bound for $\log(n!)$ bounded by a constant $c' \in \mathbb{R}$, it was already an obvious contradiction.

Since have once again stumbled upon a contradiction and clearly showed that n is bounded by a constant, we therefore proved that:

$$\log(n!) \not\in O(\log(n))$$

Now since $n\sqrt{n}$ is at most $O(n^3)$, the entire product $n\sqrt{n}\log(n!)$ will grow faster than all of the functions in the set $O(n^3\log(n))$ because:

1. $n\sqrt{n}$ is bounded by n^3
2. But $\log(n!)$ grows much faster than $\log(n)$
3. Therefore the product $n\sqrt{n}\log(n!)$ cannot be bounded by in $n^3\log(n)$.

In conclusion, this shows that:

$$n\sqrt{n}\log(n!) \not\in O(n^3\log(n))$$

Question 2

Using the limit rule, we are asked to determine the relative order (O , Ω or Θ) of the following functions:

1. $f(n) = \frac{n}{\sqrt[3]{n}}, g(n) = \ln \sqrt{n}$
2. $f(n) = 2^{bn}, g(n) = 3^n$ where $b \geq \mathbb{N}^{\geq 2}$

The limit rule states that:

$$\lim_{n \rightarrow +\infty} \frac{f(n)}{g(n)} = \begin{cases} 0 \rightarrow f(n) \in O(g(n)) \\ k \in \mathbb{R}^+ \rightarrow f(n) \in O(g(n)), g(n) \in O(f(n)) \\ +\infty \rightarrow f(n) \not\in O(g(n)), g(n) \in O(f(n)) \end{cases}$$

Let's start with the question 1:

$$\lim_{n \rightarrow +\infty} \frac{\frac{n}{\sqrt[3]{n}}}{\ln \sqrt{n}} \quad (1.1)$$

$$(*) \frac{n}{\sqrt[3]{n}} = n^{1-\frac{1}{3}} = n^{\frac{2}{3}} \rightarrow \lim_{n \rightarrow +\infty} \frac{n^{\frac{2}{3}}}{\ln \sqrt{n}} \quad (1.2)$$

$$= \lim_{n \rightarrow +\infty} \frac{n^{\frac{2}{3}}}{\frac{1}{2} \ln n} \stackrel{\text{RH}}{=} \lim_{n \rightarrow +\infty} \frac{\frac{2}{3} n^{-\frac{1}{3}}}{\frac{1}{2n}} \quad (1.3)$$

$$= \lim_{n \rightarrow +\infty} \frac{2}{3n^{\frac{1}{3}}} \times 2n = \lim_{n \rightarrow +\infty} \frac{4n}{3n^{\frac{1}{3}}} = \lim_{n \rightarrow +\infty} \frac{4n^{1-\frac{1}{3}}}{3} = \lim_{n \rightarrow +\infty} \frac{4}{3} n^{\frac{2}{3}} \quad (1.4)$$

$$= \frac{4}{3} \lim_{n \rightarrow +\infty} n^{\frac{2}{3}} = +\infty \quad (1.5)$$

$$\text{Now since: } \lim_{n \rightarrow +\infty} \frac{n^{\frac{2}{3}}}{\frac{1}{2} \ln n} = +\infty$$

Therefore, by the limit rule:

$$\ln(\sqrt{n}) \in O\left(\frac{n}{\sqrt[3]{n}}\right)$$

Continuing with question 2:

$$\lim_{n \rightarrow +\infty} \frac{2^{bn}}{3^n}, \text{ where } b \geq \mathbb{N}^{\geq 2} \quad (1.6)$$

Notice here that because $b \geq 2 \in \mathbb{N}$:

$$2^{bn} \geq 3^n, \forall n \geq 1 \quad (1.7)$$

The term $\left(\frac{2^b}{3}\right) > 1, \forall b \geq 2 \in \mathbb{N}$, so:

$$\lim_{n \rightarrow +\infty} \frac{2^{bn}}{3^n} = \lim_{n \rightarrow +\infty} \left(\frac{2^b}{3}\right)^n = +\infty \quad (1.8)$$

Therefore, for any $b \geq 2 \in \mathbb{N}$, by the limit rule:

$$3^n \in O(2^{bn})$$

Question 3

We are asked to show that $f(n) = 2n^2 - \sin(n)$ is an eventually non decreasing function (E.N.D).

For it to be E.N.D, there needs to be number $k_0 \in \mathbb{N}^*$, a threshold such that:

$$\forall n \geq k_0 \rightarrow f(n+1) \geq f(n)$$

That means that from that number k_0 :

$$f(n+1) - f(n) \geq 0, \forall n \geq k_0$$

$$\underbrace{2(n+1)^2 - \sin(n+1)}_{f(n+1)} - \underbrace{[2n^2 - \sin(n)]}_{f(n)} \quad (1.1)$$

$$\underbrace{2(n^2 + 2n + 1) - \sin(n+1)}_{f(n+1)} - \underbrace{[2n^2 - \sin(n)]}_{f(n)} \quad (1.2)$$

$$2n^2 + 4n + 2 - \sin(n+1) - 2n^2 + \sin(n) \quad (1.3)$$

That means that the following expression has to be greater than zero:

$$4n + 2 + \sin(n) - \sin(n+1) \geq 0 \quad (1.4)$$

$$\text{First, we can see that: } 4n + 2 \geq 2 \quad (1.5)$$

Also, the sine function is bounded:

$$-1 \leq \sin(n) \leq 1 \quad (1.6)$$

$$-1 \leq \sin(n+1) \leq 1 \quad (1.7)$$

Combining both sine terms:

$$-2 \leq \sin(n+1) - \sin(n) \leq 2 \quad (1.8)$$

Adding the remaining term $4n + 2$ to complete the operation:

$$4n \leq 4n + 2 + \sin(n+1) - \sin(n) \leq 4n + 4 \quad (1.9)$$

Therefore:

$$f(n+1) - f(n) = 4n + 2 + \sin(n+1) - \sin(n) \geq 4n \geq 4 > 0 \quad \forall n \geq 1 \quad (1.10)$$

Since we have been able to find a strictly positive lower boundary for $f(n+1) - f(n)$, we have shown that $f(n) = 2n^2 - \sin(n)$ is E.N.D.

2 Recurrences

Question 1

We are asked to solve the following recurrence by finding its characteristic polynomial, its roots with their multiplicity.

$$t_n = 4t_{n-1} - 4t_{n-2} + 4(n+1)4^n \quad (2.1)$$

We multiply by 4:

$$4 \times (t_n = 4t_{n-1} - 4t_{n-2} + 4(n+1)4^n) \quad (2.2)$$

$$4t_n = 16t_{n-1} - 16t_{n-2} + 16(n+1)4^n \quad \blacktriangle \quad (2.3)$$

Setting $n = n-1$ in the original form :

$$t_{n-1} = 4t_{n-2} - 4t_{n-3} + 4n4^{n-1} \quad (2.4)$$

We multiply by 4 again:

$$4t_{n-1} = 16t_{n-2} - 16t_{n-3} + 16n4^{n-1} \quad \blacksquare \quad (2.5)$$

Let's perform the following operation: $(\blacktriangle) - (\blacksquare)$

$$4t_n = 16t_{n-1} - 16t_{n-2} + 16(n+1)4^n \quad (2.6)$$

—

$$4t_{n-1} = 16t_{n-2} - 16t_{n-3} + 16n4^{n-1}$$

=

$$4t_n - 4t_{n-1} = 16t_{n-1} - 16t_{n-2} + 16(n+1)4^n - (16t_{n-2} - 16t_{n-3} + 16n4^{n-1}) \quad (2.7)$$

$$4t_n - 4t_{n-1} = 16t_{n-1} - 16t_{n-2} + 16(n+1)4^n - 16t_{n-2} + 16t_{n-3} - 16n4^{n-1} \quad (2.8)$$

$$4t_n - 4t_{n-1} - 16t_{n-1} + 32t_{n-2} - 16t_{n-3} = 16n.4^n + 16.4^n - 16n\frac{4^n}{4} \quad (2.9)$$

$$4t_n - 4t_{n-1} - 16t_{n-1} + 32t_{n-2} - 16t_{n-3} = 16 \left[n4^n - n\frac{4^n}{4} + 4^n \right] \quad (2.10)$$

$$4t_n - 4t_{n-1} - 16t_{n-1} + 32t_{n-2} - 16t_{n-3} = 16n4^n - 16n\frac{4^n}{4} + 16.4^n \quad (2.11)$$

$$4t_n - 4t_{n-1} - 16t_{n-1} + 32t_{n-2} - 16t_{n-3} = 16n4^n - 4n4^n + 16.4^n \quad (2.12)$$

$$4t_n - 20t_{n-1} + 32t_{n-2} - 16t_{n-3} = 12n4^n + 16.4^n \quad (2.13)$$

We end up with this linear recurrence. The non-homogeneous part are the terms:

$$12n4^n + 16.4^n \quad (2.14)$$

The characteristic polynomial of the recurrence (2.17) is:

$$4x^3 - 20x^2 + 32x - 16 \quad (2.15)$$

Great, let's find the solutions for the homogeneous part first, meaning all solutions that satisfy $P(x) = 0$.

$$4x^3 - 20x^2 + 32x - 16 = 0 \text{ multiply by } 1/4 \quad (2.16)$$

$$P(x) = x^3 - 5x^2 + 8x - 4 = 0 \quad (2.17)$$

I like to use ruffini's method to perform division. Although, for that we need to know a root of the polynomial. Let's try $x = 1$:

$$1^3 - 5^2 + 8 - 4 = 0 \quad (2.18)$$

$$24 + 4 \neq 0 \rightarrow x = 1 \text{ is not a root}$$

Let's try $x = 2$:

$$2^3 - 5.2^2 + 8.2 - 4 = 0 \quad (2.19)$$

$$8 - 4 - 4 = 0 \rightarrow x = 2 \text{ is a root}$$

Great, now we know that $(x - 2)$ is a factor of $P(x)$, we can perform the division using Ruffini's method. We put the coefficients of the dividend $P(x)$ in the first line, and the divisor on the left, in this case 2. We then follow Ruffini's method:

2	1	-5	8	-4
+	↓	2	-6	4
	1	-3	2	0

$$\text{We end up with: } x^2 - 3x + 2 \quad (2.20)$$

$$\Delta = b^2 - 4ac = (-3)^2 - 4(1)(2) = 9 - 8 = 1 \quad (2.21)$$

$$r_{1,2} = \frac{-b \pm \sqrt{\Delta}}{2a}$$

$$r_1 = 2, r_2 = 1 \quad (2.22)$$

$$\text{Therefore, } P(x) = (x - 2)(x - 2)(x - 1) \quad (2.23)$$

$$x = 2 \text{ with multiplicity of } 2 \quad (2.24)$$

$$x = 1 \text{ with a multiplcty of } 1 \quad (2.25)$$

So the general solution t_n^{hom} for the homogeneous part is:

$$t_n^{\text{hom}} = (c_1 + c_2 n)2^n \quad (2.26)$$

Now for the non-homogenous part, because 4^n does not correspond to a root of $P(x)$, it means that 4 is not a solution of $P(x)$.

The non-homogeneous term has $(n + 1)$ in front, which is a polynomial of degree 1 and because $x = 4$ is not a root, we do not need to multiply by extra powers of n (to make it independant). Therefore, we are looking for a solution in the form:

$$t_n^{\text{P sol}} = (An + B)4^n \quad (2.27)$$

Let's plug $t_n^{\text{P sol}}, t_{n-1}^{\text{P sol}}$ and $t_{n-2}^{\text{P sol}}$ into our original recurrence: $t_n - 4t_{n-1} + 4t_{n-2} = 4(n + 1)4^n$

$$t_n^{\text{P sol}} = (An + B)4^n \quad (2.28)$$

$$t_{n-1}^{\text{P sol}} = [A(n - 1) + B]4^{n-1} \quad (2.29)$$

$$t_{n-2}^{\text{P sol}} = [A(n - 2) + B]4^{n-2} \quad (2.30)$$

Now let's compute each term of the recurrence:

$$t_n = (An + B)4^n \quad (2.31)$$

$$-4t_{n-1} = -[A(n - 1) + B]4^n \quad (2.32)$$

$$4t_{n-2} = [A(n - 2) + B]4^{n-1} \quad (2.33)$$

Combining all terms:

$$t_n - 4t_{n-1} + 4t_{n-2} = 4(n + 1)4^n \quad (2.34)$$

$$= \quad (2.35)$$

$$(An + B)4^n - [A(n - 1) + B]4^n + [A(n - 2) + B]4^{n-1} \quad (2.36)$$

$$4^n(An + B - A(n - 1) - B) + [A(n - 2) + B]4^{n-1} \quad (2.37)$$

$$4^n(\cancel{An} + \cancel{B} - \cancel{An} + A - \cancel{B}) + [A(n - 2) + B]4^{n-1} \quad (2.38)$$

$$= A.4^n + [A(n - 2) + B]4^{n-1} \quad (2.39)$$

$$= 4^{n-1}[4A + A(n - 2) + B] \quad (2.40)$$

$$= 4^{n-1}[4A + An - 2A + B] \quad (2.41)$$

$$= 4^{n-1}[An + 2A + B] \quad (2.42)$$

After replacing every term, we end up with:

$$4^{n-1}[An + 2A + B] = (n + 1)4^{n+1} \quad (2.43)$$

$$4^n \frac{1}{4}[An + 2A + B] = 4(n + 1)4^n \quad (2.44)$$

$$\left[4^n \frac{1}{4}[An + 2A + B] = 4(n + 1)4^n \right] \times \frac{1}{4^n} \quad (2.45)$$

$$\frac{1}{4}[An + 2A + B] = 4(n + 1) \quad (2.46)$$

$$An + 2A + B = 16(n + 1) \quad (2.47)$$

$$\underbrace{An}_{\deg=1} + \underbrace{(2A + B)}_{\deg=0} = \underbrace{16n}_{\deg=1} + \underbrace{16}_{\deg=0} \quad (2.48)$$

We have the following system of equation:

$$An = 16n \quad (2.49)$$

$$2A + B = 16 \quad (2.50)$$

$$An = 16n \rightarrow A = 16 \quad (2.51)$$

$$2 \times \underbrace{16}_A + B = 16 \quad (2.52)$$

$$32 + B = 16 \quad (2.53)$$

$$B = -16 \quad (2.54)$$

We have found a valid particular solution:

$$t_n^{\text{P.sol}} = \left(\underbrace{16n}_A - \underbrace{16}_B \right) 4^n \quad (2.55)$$

Combining $t_n^{\text{hom}} + t_n^{\text{P.sol}}$ to get t_n :

$$t_n = (c_1 + c_2 n)2^n + 16(n - 1)4^n \quad (2.56)$$

Question 2

For this question, we are asked to analyze the complexity of a little python program that is recursive. I only took the portion of the code that is relevant for solving this problem - which are only the parts of the code where the method `<<t.forward(length)>>` is called.

```

1 def tree(length, level):
2     global count
3     if level > 0 :
4         t.forward(length)
5         tree(length/alpha, level - 1)
6         tree(length/alpha, level - 1)
7         tree(length/alpha, level - 1)
8
9 tree(200,4)

```

Let's start with the base case, for the level $n = 0$, `<<if level > 0: t.forward(length)>>` is not called, that means $T(0) = 0$. Furthermore, we can see that for a level $n > 0$, we are going to call `<<t.forward(length)>>` exactly once and then call recursively our tree method to draw a tree that is one unit smaller than the last level 3 times until we reach the base case where $n = 0$ - where `<<t.forward(length)>>` is not called at all. Formalizing this mathematically, we get:

$$t(n) = \begin{cases} 0 & \text{if } n = 0 \\ 3t(n-1) + 1 & \text{if } n > 1 \end{cases} \quad (2.1)$$

For a level $k \geq 1$:

$$t(k) = 1 + 3t(k-1) = 1 + 3 \times [1 + 3t(k-2)] = 1 + 3 + 3^2 \times t(k-3) \quad (2.2)$$

$$= 1 + 3 + 3^2[1 + 3t(k-4)] \quad (2.3)$$

$$1 + 3^2 + 3^3 + \dots + 3^{k-1} + 3^k \times t(0) \quad (2.4)$$

$$= 3^{k-1} + 3^k \times 0 = 3^{k-1} \quad (2.5)$$

$$\sum_{k=1}^{n-1} 3^k = \frac{r^n - 1}{r - 1} = \frac{3^n - 1}{3 - 1} = \frac{3^n - 1}{2} \quad (2.6)$$

$$\Theta\left(\frac{3^n - 1}{2}\right) = \Theta\left(\max\left(\frac{3^n - 1}{2}\right)\right) \quad (2.7)$$

$$= \Theta(3^n) \quad (2.8)$$

To conclude, the complexity of the program when we are strictly looking at the calls of the `<<t.forward(length)>>` method is in $\Theta(3^n)$.

Question 3

We are tasked to give the complexity of some recurrences using the master theorem.

Note: I will use the notation $\log_2(n) = \lg(n)$.

The master theorem:

$$\text{Let } n_0 \geq 1 \in \mathbb{N}, \ell \geq 1, b \geq 2 \in \mathbb{N}, k \geq 0 \in \mathbb{N}, c \in \mathbb{R}^+ \quad (2.9)$$

$$T(n) = \ell T\left(\frac{n}{b}\right) + cn^k, \forall n \geq n_0 \quad (2.10)$$

where $\frac{n}{n_0}$ is a power of b and $T(n)$ is E.N.D. We have:

$$T(n) \in \begin{cases} \Theta(n^k) & \text{if } \ell < b^k \\ \Theta(n^k \log_b n) & \text{if } \ell = b^k \\ \Theta(n^{\log_b \ell}) & \text{if } \ell > b^k \end{cases} \quad (2.11)$$

$$1. \ t(n) = t\left(\frac{n}{2}\right) + 4n :$$

$$\ell = 1, b = 2, k = 1, 1 < 2^1 : \text{since } \ell < b^k \rightarrow t(n) \in \Theta(n) \quad (2.12)$$

$$2. \ t(n) = 2t\left(\frac{n}{2}\right) + 2n$$

$$\ell = 2, b = 2, k = 1, 2 = 2^1 : \text{since } \ell = b^k \rightarrow t(n) \in \Theta(n \lg(n)) \quad (2.13)$$

$$3. \ t(n) = 3t\left(\frac{n}{3}\right) + 3n^3$$

$$\ell = 3, b = 3, k = 3, 3 < 3^3 : \text{since } \ell < b^k \rightarrow t(n) \in \Theta(n^3) \quad (2.14)$$

$$4. \ t(n) = 4t\left(\frac{n}{3}\right) + 2n$$

$$\ell = 4, b = 3, k = 1, 4 > 3^1 : \text{since } \ell > b^k \rightarrow t(n) \in \Theta(n^{\log_3(4)}) \approx \Theta(n^{1.2618...}) \quad (2.15)$$

$$5. \ t(n) = 4t\left(\frac{n}{2}\right) + 2n^2$$

$$\ell = 4, b = 2, k = 2, 4 = 2^2 : \text{since } \ell = b^k \rightarrow t(n) \in \Theta(n^2 \lg(n)) \quad (2.16)$$

